@prefix : <http://mobi.com/ontologies/delimited#> .
@prefix owl: <http://www.w3.org/2002/07/owl#> .
@prefix rdf: <http://www.w3.org/1999/02/22-rdf-syntax-ns#> .
@prefix xml: <http://www.w3.org/XML/1998/namespace> .
@prefix xsd: <http://www.w3.org/2001/XMLSchema#> .
@prefix rdfs: <http://www.w3.org/2000/01/rdf-schema#> .
@prefix dct: <http://purl.org/dc/terms/>.
@prefix mcat: <http://mobi.com/ontologies/catalog#> .

<http://mobi.com/ontologies/delimited> a owl:Ontology ;
    owl:imports <http://mobi.com/ontologies/catalog> ;
    owl:versionIRI <http://mobi.com/ontologies/delimited#1.0>;
    rdfs:label "The Mobi Delimited Ontology"@en ;
    rdfs:comment "The Mobi delimited ontology defines Mobi Mappings and their records in the Mobi catalog."@en ;
    dct:creator [foaf:name "Bryan Miller"], [foaf:name "Megan Mercer"];
    foaf:maker [foaf:name "Mobi"; foaf:homepage <https://mobi.inovexcorp.com/>];
    dct:modified "2017-10-06"^^xsd:date.

# MappingRecord

:MappingRecord a owl:Class;
    rdfs:subClassOf mcat:VersionedRDFRecord;
    rdfs:label "Mapping Record"@en;
    rdfs:comment "A collection of RDF data that defines a mapping resource."@en.

# Mapping

:Mapping rdf:type owl:Class ;
    rdfs:label "Mapping"@en ;
    rdfs:comment "An object that represents a mapping configuration."@en .

:sourceOntology a owl:ObjectProperty, owl:FunctionalProperty ;
    rdfs:domain :Mapping ;
    rdfs:range owl:Ontology ;
    rdfs:label "source ontology"@en ;
    rdfs:comment "Defines the ontology that the Mapping is based on."@en .

:sourceRecord a owl:ObjectProperty, owl:FunctionalProperty ;
    rdfs:domain :Mapping ;
    rdfs:range mcat:OntologyRecord ;
    rdfs:label "source record"@en ;
    rdfs:comment "Defines the OntologyRecord that the Mapping is based on."@en .

:sourceBranch a owl:ObjectProperty, owl:FunctionalProperty ;
    rdfs:domain :Mapping ;
    rdfs:range mcat:Branch ;
    rdfs:label "source branch"@en ;
    rdfs:comment "Defines the Branch of the OntologyRecord that the Mapping is based on."@en .

:sourceCommit a owl:ObjectProperty, owl:FunctionalProperty ;
    rdfs:domain :Mapping ;
    rdfs:range mcat:Commit ;
    rdfs:label "source commit"@en ;
    rdfs:comment "Defines the Commit of the OntologyRecord that the Mapping is based on."@en .

:versionIRI a owl:ObjectProperty, owl:FunctionalProperty ;
    rdfs:domain :Mapping ;
    rdfs:range xsd:anyURI ;
    rdfs:label "version IRI"@en ;
    rdfs:comment "The IRI of the current version of a Mapping."@en .

:defaultPrefix a owl:DatatypeProperty ;
    rdfs:subPropertyOf owl:topDataProperty ;
    rdfs:domain :Mapping ;
    rdfs:range xsd:string ;
    rdfs:label "default prefix"@en ;
    rdfs:comment "The default prefix used for the Mapping"@en .

# ClassMapping

:ClassMapping a owl:Class ;
    rdfs:label "Class Mapping"@en ;
    rdfs:comment "An object that represents the creation of a specific type of individual."@en .

:dataProperty a owl:ObjectProperty ;
    rdfs:subPropertyOf :propertyMapping ;
    rdfs:domain :ClassMapping ;
    rdfs:range :DataMapping ;
    rdfs:label "data property"@en ;
    rdfs:comment "A data property mapping for a ClassMapping."@en .

:mapsTo a owl:ObjectProperty ;
    rdfs:domain :ClassMapping ;
    rdfs:range owl:Thing ;
    rdfs:label "maps to"@en ;
    rdfs:comment "Defines the type that will be used when defining an object from this class mapping"@en .

:objectProperty a owl:ObjectProperty ;
    rdfs:subPropertyOf :propertyMapping ;
    rdfs:domain :ClassMapping ;
    rdfs:range :ObjectMapping ;
    rdfs:label "object property"@en ;
    rdfs:comment "An object property mapping for a ClassMapping."@en .

:hasPrefix a owl:DatatypeProperty ;
    rdfs:domain :ClassMapping ;
    rdfs:range xsd:string ;
    rdfs:label "has prefix"@en ;
    rdfs:comment "The prefix used if the Cell is an instance"@en .

:localName a owl:DatatypeProperty, owl:FunctionalProperty ;
    rdfs:domain :ClassMapping ;
    rdfs:range xsd:string ;
    rdfs:label "local name"@en ;
    rdfs:comment "The pattern specifying the local name of the generated instance. A value of \"${UUID}\" results in the generation of random UUID. A digit value results in the value for the cell in that column being inserted into the IRI (e.g. ${2} would be the value for the third column in the row)"@en .

# PropertyMapping

:PropertyMapping a owl:Class ;
    rdfs:label "Property Mapping"@en ;
    rdfs:comment "An object used to relate a ClassMapping to a property on the generated instance."@en .

# ObjectMapping

:ObjectMapping a owl:Class ;
    rdfs:subClassOf :PropertyMapping ;
    rdfs:label "Object Mapping"@en ;
    rdfs:comment "An object used to relate a ClassMapping to an Object Property on the generated instance."@en .

:classMapping a owl:ObjectProperty ;
    rdfs:domain :ObjectMapping ;
    rdfs:range :ClassMapping ;
    rdfs:label "class mapping"@en ;
    rdfs:comment "The ClassMapping that describes the target resource."@en .

# DataMapping

:DataMapping a owl:Class ;
    rdfs:subClassOf :PropertyMapping ;
    rdfs:label "Data Mapping"@en ;
    rdfs:comment "An object used to relate a ClassMapping to a Datatype Property on the generated instance."@en .

:datatypeSpec a owl:ObjectProperty, owl:FunctionalProperty ;
    rdfs:domain :DataMapping ;
    rdfs:range rdfs:Datatype ;
    rdfs:label "datatype specification"@en ;
    rdfs:comment "A datatype specification indicating what datatype to assign to a data property." .

:languageSpec a owl:DatatypeProperty, owl:FunctionalProperty ;
    rdfs:domain :DataMapping ;
    rdfs:range xsd:language ;
    rdfs:label "language specification"@en ;
    rdfs:comment "A language specification indicating what language to assign to a data property." .

# Misc.

:hasProperty a owl:ObjectProperty ;
	rdfs:domain :DataMapping, :ObjectMapping , :PropertyMapping ;
	rdfs:range rdf:Property ;
    rdfs:label "has property"@en ;
	rdfs:comment "The Property defines the relationship for the PropertyMapping"@en .

:columnIndex a owl:DatatypeProperty ;
    rdfs:domain :Cell, :DataMapping, :ObjectMapping ;
    rdfs:range xsd:integer ;
    rdfs:label "column index"@en ;
    rdfs:comment "The cells column. Starting at 0."@en .

:propertyMapping a owl:ObjectProperty ;
    rdfs:range :PropertyMapping ;
    rdfs:label "property mapping"@en ;
    rdfs:comment "A property mapping, either data or object, for a ClassMapping."@en .

rdf:Property a owl:Class .
