@prefix rdf: <http://www.w3.org/1999/02/22-rdf-syntax-ns#> .
@prefix rdfs: <http://www.w3.org/2000/01/rdf-schema#> .
@prefix owl: <http://www.w3.org/2002/07/owl#> .
@prefix xsd: <http://www.w3.org/2001/XMLSchema#> .
@prefix foaf: <http://xmlns.com/foaf/0.1/> .
@prefix dct: <http://purl.org/dc/terms/> .
@prefix prov: <http://www.w3.org/ns/prov#> .
@prefix sh: <http://www.w3.org/ns/shacl#> .
@prefix mprov: <http://mobi.com/ontologies/prov#> .
@prefix mcat: <http://mobi.com/ontologies/catalog#> .
@prefix vfs: <http://mobi.com/ontologies/documents#> .
@prefix wf: <https://mobi.solutions/ontologies/form#>.
@prefix : <http://mobi.solutions/ontologies/workflows#> .
@base <http://mobi.solutions/ontologies/workflows> .

<http://mobi.solutions/ontologies/worklows/triggers> a owl:Ontology ;
    owl:versionIRI <http://mobi.solutions/ontologies/workflows/triggers#1.0> ;
    owl:imports <http://mobi.com/ontologies/prov>, <http://mobi.com/ontologies/documents> ;
    rdfs:label "The Mobi Workflows Trigger Ontology"@en ;
    rdfs:comment "The Mobi Workflows Trigger ontology is designed to represent collections of actions that are triggered manually, by a schedule, or by events occurring in the system."@en ;
    dct:creator [foaf:name "Khalil Savoy"] ;
    foaf:maker [foaf:name "Mobi"; foaf:homepage <https://mobi.inovexcorp.com/>] ;
    dct:modified "2023-09-15"^^xsd:date .

# ScheduledTrigger

:ScheduledTrigger a owl:Class, sh:NodeShape, rdfs:Class ;
    rdfs:subClassOf :Trigger ;
    rdfs:label "Scheduled Trigger"@en ;
    rdfs:comment "A specification for executing a Workflow on a specified schedule."@en ;
    sh:property :cronExpressionPropertyShape .

:cronExpressionPropertyShape a sh:PropertyShape;
    wf:usesFormField wf:TextInput ;
    sh:path :cron ;
    sh:datatype xsd:string ;
    sh:minCount 1 ;
    sh:maxCount 1 ;
    sh:pattern "(((\d+,)+\d+|(\d+(\/|-)\d+)|\d+|\*|\?) ?){5,7}" .

:cron a owl:DatatypeProperty, owl:FunctionalProperty ;
    rdfs:label "cron"@en ;
    rdfs:comment "A cron expression that dictates when the ScheduledTrigger should kick off a Workflow."@en ;
    rdfs:domain :ScheduledTrigger ;
    rdfs:range xsd:string .

# CommitToBranchTrigger

:CommitToBranchTrigger a owl:Class, sh:NodeShape, rdfs:Class ;
    rdfs:subClassOf :EventTrigger ;
    rdfs:label "Commit to Branch Trigger"@en ;
    rdfs:comment "A specification for executing a Workflow when a Commit is made on a specified Branch of a specific Record."@en ;
    sh:property :watchesRecordPropertyShape, :watchesBranchPropertyShape .

:watchesRecordPropertyShape a sh:PropertyShape;
    wf:usesFormField wf:TextInput ;
    sh:path :watchesRecord ;
    sh:nodeKind sh:IRI ;
    sh:minCount 1 ;
    sh:maxCount 1 .

:watchesBranchPropertyShape a sh:PropertyShape;
    wf:usesFormField wf:TextInput ;
    sh:path :watchesBranch ;
    sh:nodeKind sh:IRI ;
    sh:minCount 1 ;
    sh:maxCount 1 .

:watchesRecord a owl:ObjectProperty, owl:FunctionalProperty ;
    rdfs:label "watches Record"@en ;
    rdfs:comment "The VersionedRdfRecord with the Branch to watch for Commit activity."@en ;
    rdfs:domain :CommitToBranchTrigger ;
    rdfs:range mcat:VersionedRdfRecord .

:watchesBranch a owl:ObjectProperty, owl:FunctionalProperty ;
    rdfs:label "watches Branch"@en ;
    rdfs:comment "The Branch to watch for Commit activity."@en ;
    rdfs:domain :CommitToBranchTrigger ;
    rdfs:range mcat:Branch .
